src/Language.v
@@ -1,21 +1,21 @@
 (* Celsius project *)
 (* Clément Blaudeau - Lamp@EPFL & Inria 2020-2022 *)
 (* ------------------------------------------------------------------------ *)
-
-(** This file defines all the basic structures of the language (as inductive types). *)
+(* This file defines all the basic structures of the language (as inductive types) *)
 
 Require Export List Ensembles.
 Import ListNotations.
 
+(* ------------------------------------------------------------------------ *)
 (** * Language structures *)
 
-(** ** Basic types *)
+(* Basic types *)
 Definition Var : Type := nat.
-Variant Mtd : Type := mtd(n: nat).
 Definition Loc : Type := nat.
+Variant Mtd : Type := mtd(n: nat).
 Variant ClN : Type := cln(n: nat).
 
-(** ** Expression constructors *)
+(* Expression constructors *)
 Inductive Expr: Type :=
 | e_var   : Var -> Expr
 | e_this
@@ -24,32 +24,31 @@ Inductive Expr: Type :=
 | e_new   : ClN -> (list Expr) -> Expr
 | e_asgn  : Expr -> Var -> Expr -> Expr -> Expr.
 
-(** ** Modes *)
+(* Modes *)
 Inductive Mode: Type :=
 | hot
 | warm
 | cool : nat -> Mode
 | cold.
 
-(** ** Types *)
+(* Types *)
 Notation "'Tpe'" := (prod ClN Mode).
 
-(** ** Other language constructions *)
+(* Other language constructions *)
 Variant Field   : Type := field(type: Tpe)(expr: Expr).
 Variant Method  : Type := method(μ: Mode)(args: list Tpe)(out_type: Tpe)(body: Expr).
-Variant Class   : Type := class(args: list Tpe)(fields: list Field)(methods: Mtd -> (option Method)).
+Variant Class   : Type := class(Args: list Tpe)(Flds: list Field)(Mtds: Mtd -> (option Method)).
 Variant Program : Type := program(C: list Class)(entry: Expr).
 
-(** ** Other Types *)
-Definition Value : Type := Loc.
-Definition Env: Type   := list Value.
-Definition EnvTyping: Type := list Tpe.
-Definition Obj: Type   := (ClN * Env).
-Definition Store: Type := list Obj.
+(* Other Types *)
+Definition Env         : Type := list Loc.
+Definition EnvTyping   : Type := list Tpe.
+Definition Obj         : Type := ClN * Env.
+Definition Store       : Type := list Obj.
 Definition StoreTyping : Type := list Tpe.
+Definition LocSet      : Type := Ensemble Loc.
 
-Definition LocSet := (Ensemble Loc).
-
+(* ------------------------------------------------------------------------ *)
 (** ** Global Parameters *)
 Parameter Ξ: list Class.
 Parameter Entry: ClN.
