src/Notations.v
@@ -2,13 +2,20 @@
 (* Clément Blaudeau - Lamp@EPFL & Inria 2020-2022 *)
 (* ------------------------------------------------------------------------ *)
 
+(* This file gathers all the notations used in the project. Some notations are overloaded, which we
+achieve by using type classes, instantiated when necessary. The levels are chosen carefully to allow
+notations with the same prefix to co-exist peacefully. *)
+
+(* ------------------------------------------------------------------------ *)
 From Celsius Require Export Language.
 Require Export PeanoNat.
 Export ListNotations.
 Global Open Scope nat_scope.
 Global Open Scope list_scope.
 
+(* ------------------------------------------------------------------------ *)
 (** ** Overloaded notations *)
+
 Class notation_dash (A B: Type) :=
   dash_ : A -> B -> Prop.
 Notation "s ⊨ x" := (dash_ s x ) (at level 60, x at level 98).
@@ -30,8 +37,9 @@ Class notation_authority (A: Type) :=
 Notation "s ▷ s'" := (authority_ s s') (at level 60).
 
 Class notation_big_step (A B : Type) :=
-  big_step_ : A -> Store -> Env -> Value -> B -> Store -> Prop.
-Notation "'⟦' x '⟧' '(' σ ',' ρ ',' ψ ')'  '-->'  '(' y ',' σ' ')'" := (big_step_ x σ ρ ψ y σ') (at level 80, ψ at level 98).
+  big_step_ : A -> Store -> Env -> Loc -> B -> Store -> Prop.
+Notation "'⟦' x '⟧' '(' σ ',' ρ ',' ψ ')'  '-->'  '(' y ',' σ' ')'" :=
+  (big_step_ x σ ρ ψ y σ') (at level 80, ψ at level 98).
 
 Global Hint Unfold dash_: notations.
 Global Hint Unfold dash_arrow_: notations.
@@ -39,37 +47,33 @@ Global Hint Unfold dash_colon_: notations.
 Global Hint Unfold stackability_: notations.
 Global Hint Unfold big_step_: notations.
 
-
+(* ------------------------------------------------------------------------ *)
 (** ** Non-overloaded notations *)
 
-(** *** Store typing properties *)
-Reserved Notation "Σ1 ≼ Σ2" (at level 60). (* Monotonicity *)
+(* Monotonicity *)
+Reserved Notation "Σ1 ≼ Σ2" (at level 60).
 
-(** *** Store properties *)
-Reserved Notation "σ ⪨ σ'" (at level 60). (* Compatibility *)
-Reserved Notation "s ⪯ s'" (at level 60). (* Partial monotonicity *)
+(* Partial monotonicity *)
+Reserved Notation "s ⪯ s'" (at level 60).
 
-(** *** Typing *)
+(* Typing *)
 Reserved Notation "m1 ⊑ m2" (at level 40).
 Reserved Notation "T1 <: T2" (at level 40).
-Reserved Notation "( Γ , T )  ⊢ e : U " (at level 0, e, U at level 98).
-Reserved Notation "( Γ , T )  ⊩ es : Us" (at level 0, es, Us at level 98).
+Reserved Notation "( Γ , Tthis )  ⊢ e : T " (at level 0, e, T at level 98).
+Reserved Notation "( Γ , Tthis )  ⊩ es : Ts" (at level 0, es, Ts at level 98).
 
-(** *** Scoping *)
+(* Scoping *)
 Reserved Notation "( σ1 , L1 )  ⋖  ( σ2 , L2 )" (at level 0).
 Reserved Notation "( σ1 , { l } )  ⋖  ( σ2 , L2 )" (at level 0).
 Reserved Notation "( σ1 , L1 )  ⋖  ( σ2 , { l } )" (at level 0).
 Reserved Notation "( σ1 , { l1 } )  ⋖  ( σ2 , { l2 } )" (at level 0).
-Reserved Notation "σ1  ⇝ σ2 ⋖ L" (at level 99).
 
-
-(** *** Updates *)
-Reserved Notation "[ x ↦  v ] σ" (at level 0).
-Reserved Notation "[ x ⟼ v ] σ" (at level 0).
+(* Updates *)
+Reserved Notation "[ x ↦  y ] σ" (at level 0).
+Reserved Notation "[ x ⟼ y ] σ" (at level 0).
 Notation "'dom' x" := (length x) (at level 0, x at level 1).
 
-
-(** *** Sets of locations *)
+(* Sets of locations *)
 Reserved Notation "L ⪽ σ" (at level 80).
 Notation "l ∈ L" := (Ensembles.In Loc L l) (at level 80).
 Notation "L ⊆ L'" := (Included Loc L L') (at level 60).
@@ -78,10 +82,10 @@ Notation "{ l }" := (Singleton Loc l) (at level 0, l at level 99).
 Notation "L ∪ { l }" := (Union Loc L (Singleton Loc l)) (at level 80).
 Notation "{ l } ∪ L" := (Union Loc (Singleton Loc l) L) (at level 80).
 
-(** *** Store subsets *)
+(* Store subsets *)
 Reserved Notation "L ⪽ σ" (at level 80).
 Reserved Notation "{ l } ⪽ σ" (at level 80).
 
-(** *** Definitional interpreter *)
+(* Definitional interpreter *)
 Reserved Notation "⟦ e ⟧ ( σ , ρ , ψ , n )"   (at level 80, ψ at level 98, n at level 98).
 Reserved Notation "⟦_ e _⟧ ( σ , ρ , ψ , n )" (at level 80).
