src/Scopability.v
@@ -1,21 +1,15 @@
 (* Celsius project *)
 (* Clément Blaudeau - Lamp@EPFL & Inria 2020-2022 *)
 (* ------------------------------------------------------------------------ *)
-(** This file defines the notions of scoping and scoping preservation. There are more complex and
-subtle, and should not serve as an introduction to the local reasonning properties.  The main idea
-is pretty natural: to ensure that newly created objects are hot, we need to check that,
-transitively, all locations reachable from the attributes of the object are intialized. To do so, we
-need to be able to reason about the set of locations that are reachable from a set of attributes in
-a given store. Given two stores [σ] and [σ'], and two sets of locations [L] and [L'], the pair [(σ,
-L)] "scopes" [(σ',L')] if all locations reachable from [L'] in [σ'] were already reachable from [L]
-in [σ].  But as we allow to manipulate objects under initialization, we also need to consider a
-notion of "preservation" : scoping relations that are maintained when updating from one store to
-another. *)
+(* This file defines the scopability property. Given two stores [σ] and [σ'], and two sets of
+locations [L] and [L'], the pair [(σ, L)] "scopes" [(σ',L')] if all locations reachable from [L'] in
+[σ'] were already reachable from [L] in [σ]. Wellformedness conditions are needed at some point for
+reachability lemmas. *)
 From Celsius Require Export  Wellformedness.
 Implicit Type (σ: Store) (ρ ω: Env) (l: Loc) (L: LocSet) (el: list Expr).
 
-(** ** Definitions and Notations *)
-(* The scoping relation, with the hypothesis that the sets of locations are "correct" (within the stores) *)
+(* ------------------------------------------------------------------------ *)
+(** ** Definition *)
 
 Definition scopability σ σ' L L' :=
   L ⪽ σ ->
@@ -28,14 +22,11 @@ Notation "( σ1 ,  { l } )  ⋖  ( σ2 , L2 )" := (scopability σ1 σ2 {l} L2) (
 Notation "( σ1 , L1 )  ⋖  ( σ2 ,  { l } )" := (scopability σ1 σ2 L1 {l}) (at level 0).
 Notation "( σ1 ,  { l1 } )  ⋖  ( σ2 ,  { l2 } )" := (scopability σ1 σ2 {l1} {l2}) (at level 0).
 
-Local Hint Unfold scopability : scp.
-Local Hint Unfold reachability_set: scp.
-Local Hint Resolve Union_introl: scp.
-Local Hint Resolve Union_intror: scp.
-Local Hint Resolve In_singleton: core.
+Local Hint Unfold reachability_set scopability : scp.
 
+(* ------------------------------------------------------------------------ *)
 (** ** Basic results *)
-(** We first show a set of basic results about scopability. The premisses can sometime look a bit arbitrary, but they are actually fine-tuned *)
+
 Lemma scp_refl :
   forall σ L, (σ, L) ⋖ (σ, L).
 Proof.
@@ -49,7 +40,6 @@ Proof.
   unfold scopability. steps; rch_set.
   exists l0; steps; eapply H => //.
 Qed.
-(* Global Hint Resolve scp_refl2: scp. *)
 
 Lemma scp_subset :
   forall σ1 σ2 L L1 L2,
@@ -63,7 +53,6 @@ Proof with (eauto with scp lia).
   rch_set.
   exists l0; steps ...
 Qed.
-(* Global Hint Resolve scp_subset: scp. *)
 
 Lemma scp_union :
   forall σ1 σ2 L L1 L2,
@@ -90,7 +79,6 @@ Proof with (eauto with wf rch).
   unfold scopability; intros.
   inversion H4; steps...
 Qed.
-(* Global Hint Resolve scp_union_introl: scp. *)
 
 Lemma scp_union_intror :
   forall σ1 σ2 L L1 L2,
@@ -101,16 +89,6 @@ Proof with (eauto with wf rch).
   unfold scopability; intros.
   inversion H4; steps...
 Qed.
-(* Global Hint Resolve scp_union_intror: scp. *)
-
-Lemma scp_reachability:
-  forall σ l1 l2,
-    σ ⊨ l1 ⇝ l2 ->
-    (σ, {l1}) ⋖ (σ, {l2}).
-Proof with (eauto with rch).
-  unfold scopability; intros; rch_set...
-Qed.
-Global Hint Resolve scp_reachability: scp.
 
 Lemma scp_trans:
   forall σ1 σ2 σ3 L1 L2 L3,
@@ -124,45 +102,19 @@ Proof with (eauto with scp lia).
 Qed.
 Global Hint Resolve scp_trans: scp.
 
-Lemma scp_add:
-  forall σ σ' ρ' l0 l a,
-    (σ, a) ⋖ (σ', {l}) ->
-    (σ, a) ⋖ (σ', codom ρ' ∪ {l0}) ->
-    (σ, a) ⋖ (σ', codom (l::ρ') ∪ {l0}).
-Proof.
-  intros.
-  assert ((codom (l :: ρ') ∪ {l0}) = Union Loc (Singleton Loc l) ( codom ρ' ∪ {l0})). {
-      apply Extensionality_Ensembles.
-    unfold Same_set; steps; intros l'; steps;
-      inversion H1;
-      steps; eauto using Union_introl, Union_intror.
-    - inSingleton; subst. apply Union_introl; steps.
-    - inversion H2; steps.
-      + apply Union_introl; steps.
-      + inSingleton; apply Union_intror; steps. }
-  rewrite H1; eauto with scp.
-Qed.
+(* ------------------------------------------------------------------------ *)
+(** ** Scopability and reachability *)
+(* Here we link scopability and reachability. We also add two technical results about reachability
+with wellformed stores *)
 
-Lemma scp_add_env:
-  forall I v s c e0,
-    getObj s I = Some (c, e0) ->
-    v < dom s ->
-    forall σ0 L0 L2 ,
-      L0 ⪽ σ0 ->
-      L2 ⪽ s ->
-      (σ0, L0) ⋖ (s, {v}) ->
-      (σ0, L0) ⋖ (s, L2) ->
-      (σ0, L0) ⋖ ([I ↦ (c, e0 ++ [v])] (s), L2).
-Proof.
-  intros; unfold scopability; simpl; intros.
-  destruct H8; steps.
-  assert ((s ⊨ x ⇝ l) \/ ((s ⊨ x ⇝ I) /\ (s ⊨ v ⇝ l))) by
-      eauto using rch_asgn_new with lia updates.
-  steps;
-    [ eapply H4 | eapply H3] ;
-    simpl; try (eexists; split); eauto with ss.
+Lemma scp_reachability:
+  forall σ l1 l2,
+    σ ⊨ l1 ⇝ l2 ->
+    (σ, {l1}) ⋖ (σ, {l2}).
+Proof with (eauto with rch).
+  unfold scopability; intros; rch_set...
 Qed.
-Global Hint Resolve scp_add_env: scp.
+Global Hint Resolve scp_reachability: scp.
 
 Lemma rch_add_empty: forall σ C l1 l2,
     wf σ ->
@@ -188,7 +140,14 @@ Proof.
   left. exists l1; eauto.
 Qed.
 
-(** We prove some specific results on scopability in the context of assignment. The key reasonning technique is to do a case analysis on the presence of the modified entry in the reachability path. *)
+
+(* ------------------------------------------------------------------------ *)
+(** ** Scopability and assignments *)
+(* Adding new fields or new objects has an impact on the reachable sets. The conditions to preserve
+scopability are thus a bit subtle. *)
+
+(** First, we consider updating an existing field. The key reasonning technique is to do a case
+analysis on whether or not the modified entry is in the reachability path. *)
 Lemma scp_assign:
   forall σ L l v f C ω,
     getObj σ l = Some (C, ω) ->
@@ -201,6 +160,7 @@ Proof with (eauto with scp rch).
     eexists...
 Qed.
 
+(* Then, we consider adding a new field to an existing object *)
 Lemma scp_assign_new:
   forall σ σ' x v L C,
     wf σ ->
@@ -214,11 +174,50 @@ Proof with (eauto with scp rch).
     eexists...
 Qed.
 Global Hint Resolve scp_assign_new: scp.
-(** ** Evaluation-maintained results *)
 
-(** ** Main Scopability theorem *)
-(** We show the main theorem. As for wellformedness theorem, we have to make a custom proof. We use
-the results shown for initialization, lists and assignment *)
+(* ------------------------------------------------------------------------ *)
+(** ** Scopability theorem *)
+(* The key of the proof is to generalize the induction hypothesis to a superset of locations L*)
+
+Lemma subset_union_l: forall (A B C: LocSet),
+        A ⊆ B -> A ⊆ (B ∪ C).
+Proof.
+  intros;
+    intros l ?;
+      eauto with ss.
+Qed.
+Local Hint Resolve subset_union_l: ss.
+
+Lemma subset_union_r: forall (A B C: LocSet),
+        A ⊆ C -> A ⊆ (B ∪ C).
+Proof.
+  intros;
+    intros l ?;
+      eauto with ss.
+Qed.
+Local Hint Resolve subset_union_r: ss.
+
+Ltac union_assoc :=
+    repeat match goal with
+    | H:context [(?A ∪ ?B) ∪ ?C] |- _ => rewrite Union_associative in H
+    | H:_ |- context [(?A ∪ ?B) ∪ ?C] => rewrite Union_associative
+    end.
+
+Lemma union_subset : forall (A B C: LocSet),
+        A ⊆ C -> B ⊆ C -> (A ∪ B) ⊆ C.
+Proof.
+  intros;
+    intros l [ ];
+    eauto with ss.
+Qed.
+Local Hint Resolve union_subset: ss.
+
+Lemma subset_refl : forall A, A ⊆ A.
+Proof.
+  intros A l ?; done.
+Qed.
+Local Hint Resolve subset_refl: ss.
+
 Theorem scp_theorem:
 
   (forall e σ ρ ψ v σ',
@@ -239,7 +238,7 @@ Theorem scp_theorem:
         forall ω, getObj σ ψ = Some (C, ω) ->
              (forall L, L ⪽ σ -> (codom ρ ∪ {ψ}) ⊆ L -> (σ, L) ⋖ (σ', L))).
 
-Proof with (rch_set; updates; eauto 3 with scp wf rch lia).
+Proof with (rch_set; updates; eauto 3 with scp wf ss lia).
 
   apply evalP_multi_ind;
     unfold assign in * ; intros; eval_dom; eval_wf.
@@ -262,16 +261,19 @@ Proof with (rch_set; updates; eauto 3 with scp wf rch lia).
     inverts H__ln...
     + exists l0...
     + exists v1; split... apply rch_trans with v...
+      eauto with rch.
 
   - (* e = e0.m(l0) *)
     assert ((codom vl2 ∪ {v1}) ⪽ σ2); ss...
     assert (((L ∪ {v1}) ∪ codom vl2) ⪽ σ2); ss... apply ss_trans with σ...
-    intuition auto.
-    unfold scopability; steps.
-    apply H9...
-    apply H10... intros ?...
-    apply H11... intros ? [ ]...
-    exists l0; split... inverts H__ln; eauto 6 using Union.
+    intuition auto; union_assoc.
+    unfold scopability; intros.
+    apply H9; eauto with ss.
+    apply H10; eauto with ss lia.
+    apply H11; eauto with ss lia.
+    lets (l0 & H__in & ?): H14.
+    exists l0; split; inverts H__in...
+    eauto 6 using Union.
 
   - (* e = new C(l0) *)
     assert ((L ∪ {dom σ1}) ⪽ σ1 ++ [(C, [])]). { ss... apply ss_trans with σ1... }
@@ -290,23 +292,20 @@ Proof with (rch_set; updates; eauto 3 with scp wf rch lia).
       * exists l0; split... inverts H__ln...
 
   - (* e = e0.f = e1; e2 *)
-    destruct (getObj σ2 v1) as [[C ω] |] eqn: H__obj.
-    + apply scp_trans with σ1 (L∪{v1})...
-      assert (((L ∪ {v1}) ∪ {v2}) ⪽ σ2). { ss... apply ss_trans with σ... }
-      apply scp_trans with σ2 ((L∪{v1})∪{v2})... { apply IH__e2... intros ? ... }
-      assert ((((L ∪ {v1}) ∪ {v2}) ∪ {v3}) ⪽ σ3). { ss... apply ss_trans with σ... }
+    apply scp_trans with σ1 (L∪{v1})...
+    assert (((L ∪ {v1}) ∪ {v2}) ⪽ σ2). { ss... apply ss_trans with σ... }
+    apply scp_trans with σ2 ((L∪{v1})∪{v2})... { apply IH__e2... }
+    destruct (getObj σ2 v1) as [[C ω] |] eqn: H__obj...
+    + assert ((((L ∪ {v1}) ∪ {v2}) ∪ {v3}) ⪽ σ3). { steps; ss; try apply ss_trans with σ... }
       apply scp_trans with σ3 (((L∪{v1})∪{v2})∪{v3})...
+      assert ((((L ∪ {v1}) ∪ {v2}) ∪ {v3}) ⪽ σ3). { ss... apply ss_trans with σ... }
       * eapply scp_trans with ([v1 ↦ (C, [x ↦ v2] (ω))] (σ2)) ((L ∪ {v1}) ∪ {v2})...
         -- ss...  apply ss_trans with σ...
         -- apply scp_assign...
-        -- apply IH__e'... ss... apply ss_trans with σ... intros ? ?; eauto using Union.
+        -- apply IH__e'... ss... apply ss_trans with σ...
       * apply scp_refl2... intros ? [ ]; eauto using Union.
-    + apply scp_trans with σ1 (L∪{v1})...
-      assert (((L ∪ {v1}) ∪ {v2}) ⪽ σ2). { ss... apply ss_trans with σ... }
-      apply scp_trans with σ2 ((L∪{v1})∪{v2})... { apply IH__e2... intros ? ... }
-      assert ((((L ∪ {v1}) ∪ {v2}) ∪ {v3}) ⪽ σ3). { ss... apply ss_trans with σ... }
-      apply scp_trans with σ3 (((L∪{v1})∪{v2})∪{v3})... {
-        apply IH__e'... intros ? ?. eauto using Union.  }
+    + assert ((((L ∪ {v1}) ∪ {v2}) ∪ {v3}) ⪽ σ3). { steps; ss; try apply ss_trans with σ... }
+      apply scp_trans with σ3 (((L∪{v1})∪{v2})∪{v3})... { apply IH__e'... }
       apply scp_refl2... intros ? [ ]; eauto using Union.
 
   - (* el = nil *)
@@ -317,7 +316,7 @@ Proof with (rch_set; updates; eauto 3 with scp wf rch lia).
     eapply scp_trans with σ1 (L ∪ {v1})...
     (* Union associativity would simplify things *)
     unfold scopability; intros.
-    apply IH__el... intros ? ...
+    apply IH__el...
     exists l0; split...
     inverts H__ln... inverts H9...
 
@@ -339,8 +338,9 @@ Proof with (rch_set; updates; eauto 3 with scp wf rch lia).
       lets (?ω & H__obj1 & ?): H__pM I H1.
       lets (?ω & H__obj2 & ?): H__pM1 I H__obj1.
       eapply IH__init; try eapply ss_trans with σ1 ...
-      * eapply wf_assign_new...
-      * intros ? ...
+      eapply wf_assign_new...
+    + eapply scp_subset...
+      ss... eapply ss_trans with σ...
 Qed.
 
 Corollary scp_theorem_expr:
