src/Typing.v
@@ -1,66 +1,60 @@
 (* Celsius project *)
 (* Clément Blaudeau - Lamp@EPFL & Inria 2020-2022 *)
 (* ------------------------------------------------------------------------ *)
+(* This file describes the typing rules *)
 
 From Celsius Require Export Helpers.
 
 
-(* Mode lattice *)
+(* ------------------------------------------------------------------------ *)
+(** ** Mode lattice and subtyping *)
+
 Inductive S_Mode: Mode -> Mode -> Prop :=
 | s_mode_refl : forall μ, μ ⊑ μ
 | s_mode_hot: forall μ, hot ⊑ μ
 | s_mode_warm: forall Ω, warm ⊑ cool Ω
-| s_mode_union: forall Ω1 Ω2, cool (Ω1 + Ω2) ⊑ cool Ω1
+| s_mode_cool: forall Ω1 Ω2, Ω2 <= Ω1 -> cool Ω1 ⊑ cool Ω2
 | s_mode_cold: forall μ, μ ⊑ cold
 where "m1 ⊑ m2" := (S_Mode m1 m2).
-Global Hint Resolve s_mode_cold s_mode_hot s_mode_warm s_mode_union s_mode_refl: typ.
+Global Hint Constructors S_Mode: typ.
+
+(* We then have basic results *)
 
 Lemma s_mode_trans: forall μ1 μ2 μ3, μ1 ⊑ μ2 -> μ2 ⊑ μ3 -> μ1 ⊑ μ3.
 Proof.
   intros.
   inversion H; steps;
-    inversion H0; steps.
-  rewrite Plus.plus_assoc_reverse.
-  eauto with typ.
+    inversion H0; eauto with typ lia.
 Qed.
 Global Hint Resolve s_mode_trans: typ.
 
-Lemma s_mode_cool: forall Ω1 Ω2, cool Ω1 ⊑ cool Ω2 <-> Ω2 <= Ω1.
-Proof.
-  split; intros.
-  - inversion H; subst; try lia.
-  - assert (Ω2+(Ω1 - Ω2) = Ω1) by lia.
-    pose proof (s_mode_union Ω2 (Ω1 - Ω2)).
-    rewrite H0 in H1.
-    assumption.
-Qed.
-Global Hint Resolve s_mode_cool: typ.
-
 (* Subtyping *)
 
-Variant S_Typ : Tpe -> Tpe -> Prop :=
-  s_typ_mode C μ1 μ2:
-    μ1 ⊑ μ2 ->
-    (C, μ1) <: (C, μ2)
+Inductive S_Typ : Tpe -> Tpe -> Prop :=
+| s_typ_mode C μ1 μ2:
+  μ1 ⊑ μ2 ->
+  (C, μ1) <: (C, μ2)
 where "T1 <: T2" := (S_Typ T1 T2).
-Ltac S_Typ:= repeat match goal with
-                    | H: _ <: _ |- _ => inverts H
-                    end.
-Global Hint Extern 1 => S_Typ: typ.
+
+Ltac S_Typ:= repeat match goal with | H: _ <: _ |- _ => inverts H end.
+Global Hint Extern 1 => S_Typ: typ. (* We want to invert subtyping as it is trivial *)
+
+(* Subtyping between lists of types *)
 
 Inductive S_Typs : (list Tpe) -> (list Tpe) -> Prop :=
 | s_typs_nil: S_Typs nil nil
 | s_typs_cons: forall Ts1 Ts2 T1 T2,
     S_Typs Ts1 Ts2 ->
     T1 <: T2 ->
-    S_Typs (T1::Ts1) (T2::Ts2).
+          S_Typs (T1::Ts1) (T2::Ts2).
 Global Hint Resolve s_typ_mode: typ.
+
+(* Basic results *)
 
 Lemma s_typ_refl:
   forall T, T <: T.
 Proof.
-  destruct T, m;
-    eapply s_typ_mode, s_mode_refl.
+  destruct T, m; eauto with typ.
 Qed.
 Global Hint Resolve s_typ_refl: typ.
 
@@ -79,12 +73,13 @@ Proof.
 Qed.
 Global Hint Resolve S_typs_refl: typ.
 
+(* We then define predicate to check that all locations of a list are hot *)
+
 Definition P_hot (T: Tpe) :=
   match T with
   | (_, hot) => True
   | _ => False
   end.
-
 Definition P_hots := Forall P_hot.
 
 Lemma P_hots_In:
@@ -93,105 +88,121 @@ Proof.
   unfold P_hots; intros; eapply Forall_forall; eauto.
 Qed.
 
+
+(* ------------------------------------------------------------------------ *)
 (** ** Expression Typing *)
 
-
-(** e can have the type U with env Γ and `this` of type T *)
 Inductive expr_typing : EnvTyping -> Tpe -> Expr -> Tpe -> Prop :=
+
+(* We have ambient subtyping *)
 | t_sub:
-    forall Γ T e U U',
-      (Γ, T) ⊢ e : U' ->
-      (U' <: U) ->
-      (Γ, T) ⊢ e : U
+    forall Γ Tthis e T T',
+      (Γ, Tthis) ⊢ e : T' ->
+      (T' <: T) ->
+      (Γ, Tthis) ⊢ e : T
 
+(* Lookup of a variable *)
 | t_var:
-    forall Γ T x U,
-      typeLookup Γ x = Some U ->
-      (Γ, T) ⊢ (e_var x) : U
+    forall Γ Tthis x T,
+      typeLookup Γ x = Some T ->
+      (Γ, Tthis) ⊢ (e_var x) : T
 
+(* Type of current object *)
 | t_this:
-    forall Γ T,
-      (Γ, T) ⊢ e_this : T
+    forall Γ Tthis,
+      (Γ, Tthis) ⊢ e_this : Tthis
 
+(* Accessing a field of an hot object gives an hot object *)
 | t_selhot:
-    forall Γ T e f C D μ,
-      (Γ, T) ⊢ e : (D, hot) ->
+    forall Γ Tthis e f C D μ,
+      (Γ, Tthis) ⊢ e : (D, hot) ->
       (fieldType D f = Some (C, μ)) ->
-      (Γ, T) ⊢ (e_fld e f) : (C, hot)
+      (Γ, Tthis) ⊢ (e_fld e f) : (C, hot)
 
+(* In other cases, accessing a defined fields give back its base type*)
 | t_selcool:
-    forall Γ T e f U D Ω,
-      (Γ, T) ⊢ e : (D, cool Ω) ->
+    forall Γ Tthis e f T D Ω,
+      (Γ, Tthis) ⊢ e : (D, cool Ω) ->
       f < Ω ->
-      (fieldType D f = Some U) ->
-      (Γ, T) ⊢ (e_fld e f) : U
+      (fieldType D f = Some T) ->
+      (Γ, Tthis) ⊢ (e_fld e f) : T
 
-| t_new:
-    forall Γ T C args Args Flds Mtds,
-      ct C = class Args Flds Mtds ->
-      (Γ, T) ⊩ args : Args ->
-      (Γ, T) ⊢ (e_new C args) : (C, warm)
-
+(* A newly created instance with hot arguments is also hot *)
 | t_new_hot:
-    forall Γ T C args argsTs Args Flds Mtds,
+    forall Γ Tthis C args argsTs Args Flds Mtds,
       ct C = class Args Flds Mtds ->
-      (Γ, T) ⊩ args : argsTs ->
+      (Γ, Tthis) ⊩ args : argsTs ->
       P_hots argsTs ->
       S_Typs argsTs Args ->
-      (Γ, T) ⊢ (e_new C args) : (C, hot)
+      (Γ, Tthis) ⊢ (e_new C args) : (C, hot)
 
+(* At least, a newly created instance is warm*)
+| t_new:
+    forall Γ Tthis C args Args Flds Mtds,
+      ct C = class Args Flds Mtds ->
+      (Γ, Tthis) ⊩ args : Args ->
+      (Γ, Tthis) ⊢ (e_new C args) : (C, warm)
+
+(* We restrict assignment to hot values to preserve monotonicity*)
 | t_block:
-    forall Γ T U e1 f e2 e3 C μ,
-      (Γ, T) ⊢ (e_fld e1 f) : (C, μ) ->
-      (Γ, T) ⊢ e2 : (C, hot) ->
-      (Γ, T) ⊢ e3 : U ->
-      (Γ, T) ⊢ (e_asgn e1 f e2 e3) : U
+    forall Γ Tthis T e1 f e2 e3 C μ,
+      (Γ, Tthis) ⊢ (e_fld e1 f) : (C, μ) ->
+      (Γ, Tthis) ⊢ e2 : (C, hot) ->
+      (Γ, Tthis) ⊢ e3 : T ->
+      (Γ, Tthis) ⊢ (e_asgn e1 f e2 e3) : T
 
-| t_call:
-    forall Γ T e m args argsT U e__m μ0 μ__m C,
-      (Γ, T) ⊢ e : (C, μ0) ->
-      μ0 ⊑ μ__m ->
-      methodInfo C m = Some (μ__m, argsT, U, e__m) ->
-      (Γ, T) ⊩ args : argsT ->
-      (Γ, T) ⊢ (e_mtd e m args) : U
-
+(* Calling a method on an hot object with hot arguments produces a hot object*)
 | t_call_hot:
-    forall Γ T e m args argTs paramTs D body μ0 μ_r C,
-      (Γ, T) ⊢ e : (C, hot) ->
+    forall Γ Tthis e m args argTs paramTs D body μ0 μ_r C,
+      (Γ, Tthis) ⊢ e : (C, hot) ->
       methodInfo C m = Some (μ0, paramTs, (D, μ_r), body) ->
-      (Γ, T) ⊩ args : argTs ->
+      (Γ, Tthis) ⊩ args : argTs ->
       P_hots argTs ->
       S_Typs argTs paramTs ->
-      (Γ, T) ⊢ (e_mtd e m args) : (D, hot)
-where  "( Γ , T )  ⊢ e : U" := (expr_typing Γ T e U)
+      (Γ, Tthis) ⊢ (e_mtd e m args) : (D, hot)
+
+(* Otherwise, it produces the base type *)
+| t_call:
+    forall Γ Tthis e m args argsT T e__m μ0 μ__m C,
+      (Γ, Tthis) ⊢ e : (C, μ0) ->
+      μ0 ⊑ μ__m ->
+      methodInfo C m = Some (μ__m, argsT, T, e__m) ->
+      (Γ, Tthis) ⊩ args : argsT ->
+      (Γ, Tthis) ⊢ (e_mtd e m args) : T
+
+where  "( Γ , Tthis )  ⊢ e : T" := (expr_typing Γ Tthis e T)
 
 with expr_list_typing: EnvTyping -> Tpe -> (list Expr) -> (list Tpe) -> Prop :=
-| t_exprs_nil: forall Γ T, expr_list_typing Γ T [] []
-| t_exprs_cons: forall Γ T Ts es Th eh,
-    (Γ, T) ⊩ es : Ts ->
-    (Γ, T) ⊢ eh : Th ->
-    (Γ, T) ⊩ (eh::es) : (Th::Ts)
-where  "( Γ , T )  ⊩ es : Us" := (expr_list_typing Γ T es Us).
+| t_exprs_nil: forall Γ Tthis, expr_list_typing Γ Tthis [] []
+| t_exprs_cons: forall Γ Tthis Ts es T e,
+    (Γ, Tthis) ⊩ es : Ts ->
+    (Γ, Tthis) ⊢ e : T ->
+    (Γ, Tthis) ⊩ (e::es) : (T::Ts)
+where  "( Γ , Tthis )  ⊩ es : Ts" := (expr_list_typing Γ Tthis es Ts).
 
 Global Hint Constructors expr_typing: typ.
 
+(* We add this lemma as if it were a rule (actually a consequence of t_selcool) *)
+
 Lemma t_selwarm:
-    forall Γ T e f U D,
-      (Γ, T) ⊢ e : (D, warm) ->
+    forall Γ Tthis e f U D,
+      (Γ, Tthis) ⊢ e : (D, warm) ->
       (fieldType D f = Some U) ->
-      (Γ, T) ⊢ (e_fld e f) : U.
+      (Γ, Tthis) ⊢ (e_fld e f) : U.
 Proof.
   eauto with typ.
 Qed.
 
+(* ------------------------------------------------------------------------ *)
 (** ** Field typing *)
+
 Definition T_Field (Γ:EnvTyping) T f :=
   match f with
   | field U e => ((nil:EnvTyping), T) ⊢ e : U
   end.
 
 Inductive T_Fields: EnvTyping -> Tpe -> (list Field) -> Prop :=
-| t_fields_nil: forall Γ T, T_Fields Γ T []
+| t_fields_nil: forall Γ Tthis, T_Fields Γ Tthis []
 | f_fields_cool_cons: forall Γ C Ω f fs,
     T_Field Γ (C, cool Ω) f ->
     T_Fields Γ (C, cool (S Ω)) fs ->
@@ -207,7 +218,9 @@ Proof with (eauto using T_Fields, T_Field with typ lia).
   - simpl in H. inverts H...
 Qed.
 
+(* ------------------------------------------------------------------------ *)
 (** ** Class typing *)
+
 Definition T_Classes := forall C,
     match (ct C) with
     | class Args Flds Mtds =>
@@ -215,7 +228,9 @@ Definition T_Classes := forall C,
           (forall m μ ρ T e, Mtds m = Some (method μ ρ T e) -> (ρ, (C, μ)) ⊢ e : T)
     end.
 
+(* ------------------------------------------------------------------------ *)
 (** ** Program typing *)
+
 Definition T_Prog :=
   match EntryClass with
   | class nil nil Mtds =>
@@ -224,11 +239,10 @@ Definition T_Prog :=
   | _ => False
   end.
 
-
-
-
-
+(* ------------------------------------------------------------------------ *)
 (** * Inversion lemmas *)
+(* Due to the ambient subtyping, we cannot invert typing judgments directly. We thus have to show
+basic inversion lemmas. *)
 
 Lemma t_this_inv:
   forall Γ U T,
@@ -294,7 +308,7 @@ Proof with (eauto with typ lia).
     repeat eexists; eauto with typ.
   - repeat eexists; steps...
   - inverts HeqE.
-    exists Args Flds Mtds argsTs hot; splits ...
+    exists Args Flds Mtds Args warm; splits ...
 Qed.
 
 Lemma t_asgn_inv:
@@ -305,111 +319,112 @@ Lemma t_asgn_inv:
         ((Γ, T__this) ⊢ e2 : (D, hot)) /\
         (μ' ⊑ μ) /\
         ((Γ, T__this) ⊢ e3 : (C, μ')).
-Proof with (eauto with typ lia).
+Proof with (eauto 3 with typ lia).
   introv H.
   remember (e_asgn e1 f e2 e3) as E.
   remember (C,μ) as T.
   gen C μ e1 f e2 e3.
-  induction H; steps;
-    repeat eexists; eauto using t_sub with typ.
+  induction H; steps.
+  - exists D, μ1, μ'; splits...
+  - exists C, μ, μ0; splits...
 Qed.
 
-
+(* ------------------------------------------------------------------------ *)
 (** ** Induction principle for typing *)
 
 Section typing_ind.
-  Variable P : forall Γ T e U, ((Γ, T) ⊢ e : U) -> Prop.
-  Variable Pl : forall Γ T el Ul, ((Γ, T) ⊩ el : Ul) -> Prop.
+  Variable P : forall Γ Tthis e U, ((Γ, Tthis) ⊢ e : U) -> Prop.
+  Variable Pl : forall Γ Tthis el Ul, ((Γ, Tthis) ⊩ el : Ul) -> Prop.
 
-  Variable P_sub: forall Γ T e U U' H__U' H__sub,
-      P Γ T e U' H__U' ->
-      P Γ T e U (t_sub Γ T e U U' H__U' H__sub).
+  Variable P_sub: forall Γ Tthis e U U' H__U' H__sub,
+      P Γ Tthis e U' H__U' ->
+      P Γ Tthis e U (t_sub Γ Tthis e U U' H__U' H__sub).
 
-  Variable P_var: forall Γ T x U H__lkp,
-      P Γ T (e_var x) U (t_var Γ T x U H__lkp).
+  Variable P_var: forall Γ Tthis x U H__lkp,
+      P Γ Tthis (e_var x) U (t_var Γ Tthis x U H__lkp).
 
-  Variable P_this: forall Γ T,
-      P Γ T e_this T (t_this Γ T).
+  Variable P_this: forall Γ Tthis,
+      P Γ Tthis e_this Tthis (t_this Γ Tthis).
 
-  Variable P_selhot: forall Γ T e f C D μ H__D H__field,
-      P Γ T e (D, hot) H__D ->
-      P Γ T (e_fld e f) (C, hot) (t_selhot Γ T e f C D μ H__D H__field).
+  Variable P_selhot: forall Γ Tthis e f C D μ H__D H__field,
+      P Γ Tthis e (D, hot) H__D ->
+      P Γ Tthis (e_fld e f) (C, hot) (t_selhot Γ Tthis e f C D μ H__D H__field).
 
-  Variable P_selcool: forall Γ T e f U D Ω H__D H__f H__field,
-      P Γ T e (D, cool Ω) H__D ->
-      P Γ T (e_fld e f) U (t_selcool Γ T e f U D Ω H__D H__f H__field).
+  Variable P_selcool: forall Γ Tthis e f U D Ω H__D H__f H__field,
+      P Γ Tthis e (D, cool Ω) H__D ->
+      P Γ Tthis (e_fld e f) U (t_selcool Γ Tthis e f U D Ω H__D H__f H__field).
 
-  Variable P_new: forall Γ T C args Args Flds Mtds H__ct H__args,
-      Pl Γ T args Args H__args ->
-      P Γ T (e_new C args) (C, warm) (t_new Γ T C args Args Flds Mtds H__ct H__args).
+  Variable P_new: forall Γ Tthis C args Args Flds Mtds H__ct H__args,
+      Pl Γ Tthis args Args H__args ->
+      P Γ Tthis (e_new C args) (C, warm) (t_new Γ Tthis C args Args Flds Mtds H__ct H__args).
 
-  Variable P_new_hot: forall Γ T C args argsTs Args Flds Mtds H__ct H__args H__hots H__subs,
-      Pl Γ T args argsTs H__args ->
-      P Γ T (e_new C args) (C, hot) (t_new_hot Γ T C args argsTs Args Flds Mtds H__ct H__args H__hots H__subs).
+  Variable P_new_hot: forall Γ Tthis C args argsTs Args Flds Mtds H__ct H__args H__hots H__subs,
+      Pl Γ Tthis args argsTs H__args ->
+      P Γ Tthis (e_new C args) (C, hot) (t_new_hot Γ Tthis C args argsTs Args Flds Mtds H__ct H__args H__hots H__subs).
 
-  Variable P_block: forall Γ T U e1 f e2 e3 C μ H__fld H__e2 H__e3,
-      P Γ T (e_fld e1 f) (C, μ) H__fld ->
-      P Γ T e2 (C, hot) H__e2 ->
-      P Γ T e3 U H__e3 ->
-      P Γ T (e_asgn e1 f e2 e3) U (t_block Γ T U e1 f e2 e3 C μ H__fld H__e2 H__e3).
+  Variable P_block: forall Γ Tthis U e1 f e2 e3 C μ H__fld H__e2 H__e3,
+      P Γ Tthis (e_fld e1 f) (C, μ) H__fld ->
+      P Γ Tthis e2 (C, hot) H__e2 ->
+      P Γ Tthis e3 U H__e3 ->
+      P Γ Tthis (e_asgn e1 f e2 e3) U (t_block Γ Tthis U e1 f e2 e3 C μ H__fld H__e2 H__e3).
 
-  Variable P_call: forall Γ T e m args argsT U e__m μ0 μ__m C H__e H__sub H__mtd H__args,
-      P Γ T e (C, μ0) H__e ->
-      Pl Γ T args argsT H__args ->
+  Variable P_call: forall Γ Tthis e m args argsT U e__m μ0 μ__m C H__e H__sub H__mtd H__args,
+      P Γ Tthis e (C, μ0) H__e ->
+      Pl Γ Tthis args argsT H__args ->
       (* P argsT (C, μ__m) e__m U (typable_method m C μ__m argsT U e__m H__mtd) ->*)
-      P Γ T (e_mtd e m args) U (t_call Γ T e m args argsT U e__m μ0 μ__m C H__e H__sub H__mtd H__args).
+      P Γ Tthis (e_mtd e m args) U (t_call Γ Tthis e m args argsT U e__m μ0 μ__m C H__e H__sub H__mtd H__args).
 
-  Variable P_call_hot: forall Γ T e m args argTs paramTs D body μ0 μ_r C H__e H__mtd H__args H__hots H__subs,
-      P Γ T e (C, hot) H__e ->
-      Pl Γ T args argTs H__args ->
-      P Γ T (e_mtd e m args) (D, hot) (t_call_hot Γ T e m args argTs paramTs D body μ0 μ_r C H__e H__mtd H__args H__hots H__subs).
+  Variable P_call_hot: forall Γ Tthis e m args argTs paramTs D body μ0 μ_r C H__e H__mtd H__args H__hots H__subs,
+      P Γ Tthis e (C, hot) H__e ->
+      Pl Γ Tthis args argTs H__args ->
+      P Γ Tthis (e_mtd e m args) (D, hot) (t_call_hot Γ Tthis e m args argTs paramTs D body μ0 μ_r C H__e H__mtd H__args H__hots H__subs).
 
-  Variable Pl_nil: forall Γ T,
-      Pl Γ T [] [] (t_exprs_nil Γ T).
+  Variable Pl_nil: forall Γ Tthis,
+      Pl Γ Tthis [] [] (t_exprs_nil Γ Tthis).
 
-  Variable Pl_cons: forall Γ T U Ul e el H__el H__e,
-      P Γ T e U H__e ->
-      Pl Γ T el Ul H__el ->
-      Pl Γ T (e::el) (U::Ul) (t_exprs_cons Γ T Ul el U e H__el H__e).
+  Variable Pl_cons: forall Γ Tthis U Ul e el H__el H__e,
+      P Γ Tthis e U H__e ->
+      Pl Γ Tthis el Ul H__el ->
+      Pl Γ Tthis (e::el) (U::Ul) (t_exprs_cons Γ Tthis Ul el U e H__el H__e).
 
-  Fixpoint typing_ind Γ T e U (typing: (Γ, T) ⊢ e : U) : P Γ T e U typing :=
+  Fixpoint typing_ind Γ Tthis e U (typing: (Γ, Tthis) ⊢ e : U) : P Γ Tthis e U typing :=
     match typing with
-    | t_sub Γ T e U U' H__U' H__sub => P_sub Γ T e U U' H__U' H__sub (typing_ind Γ T e U' H__U')
-    | t_var Γ T x U H__lkp => P_var Γ T x U H__lkp
-    | t_this Γ T => P_this Γ T
-    | t_selhot Γ T e f C D μ H__D H__field =>
-        P_selhot Γ T e f C D μ H__D H__field
-                 (typing_ind Γ T e (D, hot) H__D)
-    | t_selcool Γ T e f U D Ω H__D H__f H__field =>
-        P_selcool Γ T e f U D Ω H__D H__f H__field
-                  (typing_ind Γ T e (D, cool Ω) H__D)
-    | t_new Γ T C args Args Flds Mtds H__ct H__args =>
-        P_new Γ T C args Args Flds Mtds H__ct H__args
-              (typing_list_ind Γ T args Args H__args)
-    | t_new_hot Γ T C args argsTs Args Flds Mtds H__ct H__args H__hots H__subs =>
-        P_new_hot Γ T C args argsTs Args Flds Mtds H__ct H__args H__hots H__subs
-                  (typing_list_ind Γ T args argsTs H__args)
-    | t_block Γ T U e1 f e2 e3 C μ H__fld H__e2 H__e3 =>
-        P_block Γ T U e1 f e2 e3 C μ H__fld H__e2 H__e3
-                (typing_ind Γ T (e_fld e1 f) (C, μ) H__fld)
-                (typing_ind Γ T e2 (C, hot) H__e2)
-                (typing_ind Γ T e3 U H__e3)
-    | t_call Γ T e m args argsT U e__m μ0 μ__m C H__e H__sub H__mtd H__args =>
-        P_call Γ T e m args argsT U e__m μ0 μ__m C H__e H__sub H__mtd H__args
-               (typing_ind Γ T e (C, μ0) H__e)
-               (typing_list_ind Γ T args argsT H__args)
-    | t_call_hot Γ T e m args argTs paramTs D body μ0 μ_r C H__e H__mtd H__args H__hots H__subs =>
-        P_call_hot Γ T e m args argTs paramTs D body μ0 μ_r C H__e H__mtd H__args H__hots H__subs
-                   (typing_ind Γ T e (C, hot) H__e)
-                   (typing_list_ind Γ T args argTs H__args)
+    | t_sub Γ Tthis e U U' H__U' H__sub => P_sub Γ Tthis e U U' H__U' H__sub (typing_ind Γ Tthis e U' H__U')
+    | t_var Γ Tthis x U H__lkp => P_var Γ Tthis x U H__lkp
+    | t_this Γ Tthis => P_this Γ Tthis
+    | t_selhot Γ Tthis e f C D μ H__D H__field =>
+        P_selhot Γ Tthis e f C D μ H__D H__field
+                 (typing_ind Γ Tthis e (D, hot) H__D)
+    | t_selcool Γ Tthis e f U D Ω H__D H__f H__field =>
+        P_selcool Γ Tthis e f U D Ω H__D H__f H__field
+                  (typing_ind Γ Tthis e (D, cool Ω) H__D)
+    | t_new Γ Tthis C args Args Flds Mtds H__ct H__args =>
+        P_new Γ Tthis C args Args Flds Mtds H__ct H__args
+              (typing_list_ind Γ Tthis args Args H__args)
+    | t_new_hot Γ Tthis C args argsTs Args Flds Mtds H__ct H__args H__hots H__subs =>
+        P_new_hot Γ Tthis C args argsTs Args Flds Mtds H__ct H__args H__hots H__subs
+                  (typing_list_ind Γ Tthis args argsTs H__args)
+    | t_block Γ Tthis U e1 f e2 e3 C μ H__fld H__e2 H__e3 =>
+        P_block Γ Tthis U e1 f e2 e3 C μ H__fld H__e2 H__e3
+                (typing_ind Γ Tthis (e_fld e1 f) (C, μ) H__fld)
+                (typing_ind Γ Tthis e2 (C, hot) H__e2)
+                (typing_ind Γ Tthis e3 U H__e3)
+    | t_call Γ Tthis e m args argsT U e__m μ0 μ__m C H__e H__sub H__mtd H__args =>
+        P_call Γ Tthis e m args argsT U e__m μ0 μ__m C H__e H__sub H__mtd H__args
+               (typing_ind Γ Tthis e (C, μ0) H__e)
+               (typing_list_ind Γ Tthis args argsT H__args)
+    | t_call_hot Γ Tthis e m args argTs paramTs D body μ0 μ_r C H__e H__mtd H__args H__hots H__subs =>
+        P_call_hot Γ Tthis e m args argTs paramTs D body μ0 μ_r C H__e H__mtd H__args H__hots H__subs
+                   (typing_ind Γ Tthis e (C, hot) H__e)
+                   (typing_list_ind Γ Tthis args argTs H__args)
     end
-  with typing_list_ind Γ T el Ul (typing_list: (Γ, T) ⊩ el : Ul) : Pl Γ T el Ul typing_list :=
+  with typing_list_ind Γ Tthis el Ul (typing_list: (Γ, Tthis) ⊩ el : Ul) : Pl Γ Tthis el Ul typing_list :=
          match typing_list with
-         | t_exprs_nil Γ T => Pl_nil Γ T
-         | t_exprs_cons Γ T Ul el U e H__el H__e =>
-             Pl_cons Γ T U Ul e el H__el H__e
-                     (typing_ind Γ T e U H__e)
-                     (typing_list_ind Γ T el Ul H__el)
+         | t_exprs_nil Γ Tthis => Pl_nil Γ Tthis
+         | t_exprs_cons Γ Tthis Ul el U e H__el H__e =>
+             Pl_cons Γ Tthis U Ul e el H__el H__e
+                     (typing_ind Γ Tthis e U H__e)
+                     (typing_list_ind Γ Tthis el Ul H__el)
          end.
 
 End typing_ind.
